src/Std/Data/DHashMap/Internal/Model.lean
@@ -408,6 +408,12 @@ def insertListₘ [BEq α] [Hashable α] (m : Raw₀ α β) (l : List ((a : α) 
   | .cons hd tl => insertListₘ (m.insert hd.1 hd.2) tl
 
 /-- Internal implementation detail of the hash map -/
+def eraseListₘ [BEq α] [Hashable α] (m : Raw₀ α β) (l : List ((a : α) × β a)) : Raw₀ α β :=
+  match l with
+  | .nil => m
+  | .cons hd tl => eraseListₘ (m.erase hd.1) tl
+
+/-- Internal implementation detail of the hash map -/
 def insertListIfNewₘ [BEq α] [Hashable α] (m : Raw₀ α β) (l : List ((a : α) × β a)) : Raw₀ α β :=
   match l with
   | .nil => m
@@ -654,6 +660,20 @@ theorem insertMany_eq_insertListₘ [BEq α] [Hashable α] (m : Raw₀ α β) (l
   | nil => simp [insertListₘ]
   | cons hd tl ih =>
     simp only [List.foldl_cons, insertListₘ]
+    apply ih
+
+theorem eraseMany_eq_eraseListₘ [BEq α] [Hashable α] (m : Raw₀ α β) (l : List ((a : α) × β a)) :
+    eraseMany m l = eraseListₘ m l := by
+  simp only [eraseMany, Id.run_pure, pure_bind, List.forIn_pure_yield_eq_foldl]
+  suffices ∀ (t : { m' // ∀ (P : Raw₀ α β → Prop),
+      (∀ {m'' : Raw₀ α β} {a : α}, P m'' → P (m''.erase a)) → P m → P m' }),
+        (List.foldl (fun m' p => ⟨m'.val.erase p.1, fun P h₁ h₂ => h₁ (m'.2 _ h₁ h₂)⟩) t l).val =
+      t.val.eraseListₘ l from this _
+  intro t
+  induction l generalizing m with
+  | nil => simp [eraseListₘ]
+  | cons hd tl ih =>
+    simp only [List.foldl_cons, eraseListₘ]
     apply ih
 
 theorem insertManyIfNew_eq_insertListIfNewₘ [BEq α] [Hashable α] (m : Raw₀ α β) (l : List ((a : α) × β a)) :
